examples/dm4all/NDAngelic.fst
@@ -1,0 +1,129 @@
+module NDAngelic
+
+module List = FStar.List.Tot
+
+let repr (a:Type) = unit -> list a
+
+let return (a:Type u#a) (x:a) = fun () -> [x]
+
+let bind (a : Type u#aa) (b : Type u#bb)
+    (l : repr a) (f : a -> repr b) = fun () -> List.flatten (List.map (fun x -> f x ()) (l ()))
+
+(* let choose (#a : Type) (x y : a) : repr a = fun () -> [x;y] *)
+
+(* Angelic interpretation *)
+let interp (a:Type) (l : repr a) : pure_wp a =
+    fun p -> exists (x:a). List.memP x (l ()) /\ p x
+
+total
+reifiable
+reflectable
+new_effect {
+  ND : a:Type -> Effect
+  with
+       repr      = repr
+     ; return    = return
+     ; bind      = bind
+
+     ; wp_type   = pure_wp
+     ; return_wp = pure_return
+     ; bind_wp   = pure_bind_wp
+
+     ; interp    = interp
+
+     (* ; choose    = choose *)
+}
+
+let test1 () : ND int (fun p -> p 5 /\ p 3) = 5
+let test2 () : ND int (fun p -> p 5 /\ p 3) = 3
+
+// Whoa! This used to succeed since the effect is marked as reifiable,
+// and Rel compares the representation types on each side for the
+// subtyping. and both are just `unit -> list a`. I changed it to check
+// the WPs via stronger-than instead of always unfolding.
+[@expect_failure]
+let test3 () : ND int (fun p -> p 5 /\ p 3) = 4
+
+effect Nd (a:Type) (pre:pure_pre) (post:pure_post' a pre) =
+        ND a (fun (p:pure_post a) -> pre /\ (forall (pure_result:a). post pure_result ==> p pure_result))
+
+effect NDTot (a:Type) = ND a (pure_null_wp a)
+
+val choose : #a:Type0 -> x:a -> y:a -> ND a (fun p -> p x \/ p y)
+let choose #a x y =
+    // the VC for this is valid, but F*/Z3 won't instantiate the existential, sigh.
+    // we could prove it via tactics, but that feels rather silly to do
+    admit ();
+    ND?.reflect (fun () -> [x;y])
+
+val fail : #a:Type0 -> unit -> ND a (fun p -> False)
+let fail #a () =
+    ND?.reflect (fun () -> [])
+
+let test () : ND int (fun p -> exists (x:int). 6 <= x /\ x <= 9 /\ p x) =
+    let x = choose 0 1 in
+    let y = choose 2 3 in
+    let z = choose 4 5 in
+    x + y + z
+
+[@expect_failure]
+let test_bad () : ND int (fun p -> exists (x:int). 0 <= x /\ x < 5 /\ p x) =
+    let x = choose 0 1 in
+    let y = choose 2 3 in
+    let z = choose 4 5 in
+    x + y + z
+
+let rec pick #a (l : list a) : ND a (fun p -> exists x. List.memP x l /\ p x) =
+    match l with
+    | [] -> fail ()
+    | x::xs ->
+      // choose x (pick xs)
+      // ^ this is wrong! it will call `pick xs` before choosing and always
+      //   end up returning []
+      if choose true false
+      then x
+      else pick xs
+
+let gguard (b:bool) : ND unit (fun p -> b /\ p ()) =
+  if b
+  then ()
+  else fail ()
+
+let ( * ) = op_Multiply
+
+open FStar.Tactics
+
+(* This takes a while ... *)
+#push-options "--z3rlimit 100"
+let pyths () : ND (int & int & int) (fun p -> exists x y z. x >= 1 /\ x <= 10 /\
+                                                            y >= 1 /\ y <= 10 /\
+                                                            z >= 1 /\ z <= 10 /\
+                                                            x*x + y*y == z*z /\
+                                                            p (x,y,z))
+               by (compute (); explode ())
+             =
+  let l = [1;2;3;4;5;6;7;8;9;10] in
+  let x = pick l in
+  let y = pick l in
+  let z = pick l in
+  gguard (x*x + y*y = z*z);
+  (x,y,z)
+#pop-options
+
+(* Check ND.ml for the triples:
+
+let (pyths_norm : unit -> (Prims.int * Prims.int * Prims.int) Prims.list) =
+  fun uu____1038  ->
+    [((Prims.parse_int "3"), (Prims.parse_int "4"), (Prims.parse_int "5"));
+    ((Prims.parse_int "4"), (Prims.parse_int "3"), (Prims.parse_int "5"));
+    ((Prims.parse_int "6"), (Prims.parse_int "8"), (Prims.parse_int "10"));
+    ((Prims.parse_int "8"), (Prims.parse_int "6"), (Prims.parse_int "10"))]
+*)
+let pyths_norm () = normalize_term (reify (pyths ()) ())
+
+let test_reify_1 () = assert (reify (test1 ()) () ==  [5])
+let test_reify_2 () = assert (reify (test2 ()) () ==  [3])
+let test_reify_3 () = assert (reify (test1 ()) () =!= [4])
+
+[@expect_failure]
+let _ = assert False
